lakefile.lean
@@ -14,6 +14,9 @@ require VCVio from git "https://github.com/dtumad/VCV-io.git" @ "master"
 
 require checkdecls from git "https://github.com/PatrickMassot/checkdecls.git"
 
+-- Dependent rewrite tactic
+require seq from git "https://github.com/Vtec234/lean4-seq.git"
+
 -- meta if get_config? env = some "dev" then
 require «doc-gen4» from git "https://github.com/leanprover/doc-gen4" @ "main"
 
